pcuic/theories/PCUICClosed.v
@@ -279,7 +279,7 @@ Proof.
   - rewrite closedn_subst_instance_constr.
     eapply declared_inductive_inv in X0; eauto.
     apply onArity in X0. repeat red in X0.
-    destruct X0 as [[s Hs] _]. rewrite -> andb_and in Hs.
+    destruct X0 as [Hisa [s Hs] _]. rewrite -> andb_and in Hs.
     intuition eauto using closed_upwards with arith.
 
   - destruct isdecl as [Hidecl Hcdecl].
@@ -310,10 +310,7 @@ Proof.
     simpl. apply closedn_mkApps_inv in H2.
     rewrite forallb_rev H1. apply H2.
     rewrite closedn_subst_instance_constr.
-    destruct isdecl as [isdecl [Hpdecl Hnpar]].
-    eapply declared_inductive_inv in isdecl; eauto.
-    apply onProjections in isdecl.
-    eapply nth_error_alli in isdecl; eauto.
+    eapply declared_projection_inv in isdecl; eauto.
     red in isdecl.
     destruct decompose_prod_assum eqn:Heq.
     destruct isdecl as [[s Hs] Hc]. simpl in *.
