pcuic/theories/PCUICWeakeningEnv.v
@@ -209,15 +209,29 @@ Proof.
   simpl in *.
   destruct Hdecl as [onI onP onnP]; constructor; eauto.
   - eapply Alli_impl; eauto. intros.
-    destruct X. constructor.
-    unfold on_arity, on_type in *; intuition eauto.
-    unfold on_constructors in *. eapply Alli_impl; eauto.
+    destruct X. unshelve econstructor.
+    unfold on_constructors in *. eapply Alli_impl_trans; eauto.
     intros ik [[id t] ar]. unfold on_constructor, on_type in *; intuition eauto.
-    red in onProjections |- *.
-    eapply Alli_impl; eauto. intros ip [id trm].
-    unfold on_projection, on_type; eauto.
-    destruct decompose_prod_assum. intuition auto.
-    eapply HPΣ; eauto.
+    destruct b. exists x0.
+    -- induction (cshape_args x0); simpl in *; auto.
+       destruct a0 as [na [b|] ty]; simpl in *; intuition eauto.
+    -- destruct onArity; constructor; unfold on_type in *; intuition eauto.
+    -- intros Hprojs; destruct onProjections; try constructor; auto.
+       eapply Alli_impl; eauto. intros ip [id trm].
+       unfold on_projection, on_type; eauto.
+       destruct decompose_prod_assum. intuition auto.
+       eapply HPΣ; eauto.
+    -- unfold Alli_impl_trans. simpl.
+       destruct onkelim as [sf [Hsf Hsfle]].
+       exists sf; intuition eauto. rewrite -{}Hsf.
+       unfold elimination_topsort.
+       destruct destArity as [[ctx s]|]; simpl; auto.
+       destruct universe_family; auto.
+       revert onConstructors. generalize (ind_ctors x).
+       unfold Alli_rect.
+       intros ? onCs. depelim onCs; auto. depelim onCs; simpl; auto.
+       destruct hd as [[? ?] ?]. unfold prod_rect; simpl.
+       destruct o as [? [? ?]]. simpl. reflexivity.
   - red in onP |- *. eapply All_local_env_impl; eauto.
 Qed.
 
@@ -309,8 +323,10 @@ Proof.
   intros.
   destruct H0 as [Hidecl [Hcdecl Hnpar]].
   eapply declared_inductive_inv in Hidecl; eauto.
-  apply onProjections in Hidecl.
+  apply onProjections, on_projs in Hidecl.
   eapply nth_error_alli in Hidecl; eauto.
+  eapply nth_error_Some_length in Hcdecl.
+  destruct (ind_projs idecl); simpl in *. lia. congruence.
 Qed.
 
 Lemma wf_extends `{checker_flags} {Σ Σ'} : wf Σ' -> extends Σ Σ' -> wf Σ.
